Further simple inference testing

typing/pure_inference_testScript.sml
@@ -6,8 +6,8 @@ val _ = new_theory "pure_inference_test";
 (********************)
 
 Definition parse_and_infer_def:
-  parse_and_infer parse ns str =
-    let parsed = parse str in do
+  parse_and_infer parse ns str = do
+      parsed <<- parse str;
       (ty, as, cs) <- infer ns LN parsed;
       if ¬ null as then fail else return ();
       subs <- solve cs;
@@ -41,6 +41,34 @@ Definition solve_k_def:
         (nvs, s, scheme) <<- generalise 0 0 vs FEMPTY t2;
         solve_k n (Instantiate d t1 (nvs, scheme) :: cs) od
 End
+
+Definition parse_and_get_constraints_def:
+  parse_and_get_constraints parse ns str = do
+      parsed <<- parse str;
+      (ty, as, cs) <- infer ns LN parsed;
+      if ¬ null as then fail else return (ty, cs)
+    od 0
+End
+
+Definition parse_and_solve_k_def:
+  parse_and_solve_k k parse ns str = do
+      parsed <<- parse str;
+      (ty, as, cs) <- infer ns LN parsed;
+      if ¬ null as then fail else return ();
+      subs <- solve_k k cs;
+      return subs
+    od 0
+End
+
+val debug_eval =
+  let val cmp = pure_parse_infer_compset ()
+      val _ = computeLib.extend_compset
+                [computeLib.Defs [
+                  fetch "-" "solve_k_compute",
+                  fetch "-" "parse_and_get_constraints_def",
+                  fetch "-" "parse_and_solve_k_def"
+                  ]] cmp
+  in computeLib.CBV_CONV cmp end;
 
 Definition bool_datatype_def[simp]:
   bool_datatype : typedef = (0n, [("True", []); ("False", [])])
@@ -144,6 +172,91 @@ Theorem example_2_overall:
   return (1, Function (Function (PrimTy Bool) (TypeVar 0)) (TypeVar 0)) 5
 Proof
   simp[parse_and_infer_def] >> CONV_TAC pure_parse_infer_eval
+QED
+
+(********************)
+
+val add_str = toMLstring `
+  (letrec
+    (add (lam (x y)
+      (case x temp
+        (Z y)
+        ((S (xx)) (app add xx (cons S y))))))
+    add)`;
+
+Theorem add_str_type:
+  parse_and_infer parse_cexp simple_ns ^add_str =
+    return (0, Functions [TypeCons 2 []; TypeCons 2 []] (TypeCons 2 [])) 10
+Proof
+  simp[parse_and_infer_def] >> CONV_TAC pure_parse_infer_eval >> EVAL_TAC
+QED
+
+(********************)
+
+Definition even_nat_datatype_def[simp]:
+  even_nat_datatype odd_nat_id : typedef =
+    (0n, [("EZ", []) ;("ES", [TypeCons odd_nat_id []])])
+End
+
+Definition odd_nat_datatype_def[simp]:
+  odd_nat_datatype even_nat_id : typedef =
+    (0n, [("OS", [TypeCons even_nat_id []])])
+End
+
+Definition even_odd_ns_def[simp]:
+  even_odd_ns = (
+    [] : exndef , (* no exceptions *)
+    [even_nat_datatype 1; odd_nat_datatype 0]
+  )
+End
+
+val add_even_even_str = toMLstring `
+  (letrec
+    (add_ee (lam (e1 e2)
+      (case e1 temp1
+        (EZ e2)
+        ((ES (o1))
+          (case o1 temp1
+            ((OS (e)) (cons ES (cons OS (app add_ee e e2))))
+          )))))
+   add_ee)`;
+
+Theorem add_str_type:
+  parse_and_infer parse_cexp even_odd_ns ^add_even_even_str =
+    return (0, Functions [TypeCons 0 []; TypeCons 0 []] (TypeCons 0 [])) 12
+Proof
+  simp[parse_and_infer_def] >> CONV_TAC pure_parse_infer_eval >> EVAL_TAC
+QED
+
+val add_even_odd_nats_str = toMLstring `
+  (letrec
+    (add_ee (lam (e1 e2)
+      (case e1 temp
+        (EZ e2)
+        ((ES (o1)) (cons ES (app add_eo e2 o1))))))
+
+    (add_eo (lam (e o)
+      (case e temp
+        (EZ o)
+        ((ES (o1)) (cons OS (app add_oo o1 o))))))
+
+    (add_oo (lam (o1 o2)
+      (case o1 temp
+        ((OS (e)) e (cons ES (app add_eo e o2))))))
+
+  (cons 0 add_ee add_eo add_oo))`;
+
+(* TODO bug here:
+    add_oo is given type `odd -> α -> even` instead of `odd -> odd -> even` *)
+Theorem add_str_type:
+  parse_and_infer parse_cexp even_odd_ns ^add_even_odd_nats_str =
+    return (1, Tuple [
+      Functions [TypeCons 0 []; TypeCons 0 []] (TypeCons 0 []);
+      Functions [TypeCons 0 []; TypeCons 1 []] (TypeCons 1 []);
+      Functions [TypeCons 1 []; TypeVar 0] (TypeCons 0 []);
+      ]) 28
+Proof
+  simp[parse_and_infer_def] >> CONV_TAC pure_parse_infer_eval >> EVAL_TAC
 QED
 
 (********************)
